**rigid body motion** -- free rotation around any axis
looking at fixed axis--direction of axis is always along the same, but the axis may move.

- when a rigid body rotates, every particle in the body remains at a fixed distance from the axis.
- $|\mathbf{r}|$ is constant.
	- $\mathbf{r}$ may change if the velocity is perpendicular to $\mathbf{r}$.
	- generally, $r$ is the distance from origin
		- $r = \sqrt{x^2 + y^2 + z^2}$
		- $\rho$ denotes perpendicular distance to axis

body rotating around $z$ axis
$$|\mathbf{v}_j| = |\mathbf{\dot{r}}_j|$$
$$ = \omega\rho_j$$
because axis of rotation is the z axis, $\rho_j = \sqrt{x_j^2 + y_j^2}$
thus, $\mathbf{L}_j$:
$$\mathbf{L_j} = r_j\times m_j\mathbf{v}_j$$
since we are only concerned with $L_z$:
$$L_{j, z} = m_jv_j\rho_j$$
$$L_{j, z} = m_j\rho_j^2\omega$$
total $L_z$ is the sum of the individual $z$ components:
$$L_z = \sum_j m_j\rho_j^2\omega$$
Because the body is rigid, we assume $\omega$ is constant throughout.

## 7.3.1 moment of inertia
$$L_z = I\omega$$
where $$I = \sum_j m_j\rho_j^2$$
$I$ is known as the moment of inertia. It depends on the distribution of mass.

$L_z = I\omega$ is very similar to $P = Mv$. Moment of inertia is the equivalent to mass in a rotational system.

when matter is continuously distributed, we can turn $I$ into an integral:
$$\sum_jm_j\rho_j^2 \rightarrow \int\rho_2dm$$

$$I = \int\rho^2dm = \int(x^2 + y^2)dm$$
where $dm$ is often replaced with $wdV$, where $w$ = density
thus $$ I = \int(x^2 + y^2)w dV$$


[[simple moments of inertia]]

## 7.3.2 the parallel axis theorem
If we know $I_0$, the moment of inertia through a center of mass parallel to $I$, then we know $I$.
$$I = I_0 + Ml^2$$
[[proof of parallel axis theorem]]

in [[simple moments of inertia]], we found that the moment of inertia for a stick around the midpoint is $\frac{1}{12}ML^2$. The moment of inertia of its end, then:
$$I_a = \frac{1}{12}ML^2 + M(\frac{L}{2})^2$$
$$ = \frac{1}{3}ML^2$$
similarly, the moment of inertia of a disk around an axis at the rim:
$$I_a = \frac{1}{2}MR^2 + MR^2 = \frac{3}{2}MR^2$$

