for fixed axis rotation,
$$\mathbf{L} = I\omega$$
however, this is not necessarily true when $\mathbf{L}$ and $\omega$ are not parallel

### 8.6.1 tensor of inertia
return to considering angular momentum about the center of mass
knowing that a displacement of a rigid body can be described by the displacement of its center of mass and a rotation around some axis:
$$\mathbf{L} = \mathbf{R}\times M\mathbf{V} + \sum\mathbf{r'}_j\times m_j\mathbf{\dot{r}'}_j$$
$$\mathbf{\tau} = \mathbf{R}\times\mathbf{F} + \sum\mathbf{r'}_j\times\mathbf{f}_j$$
Since $\tau = dL/dt$:
$$\mathbf{R}\times\mathbf{F} + \sum{\mathbf{r'}_j\times\mathbf{f}_j} = \mathbf{R}\times M\mathbf{A}+\frac{d}{dt}(\sum\mathbf{r'}_j\times m_j\mathbf{\dot{r}'}_j)$$
Since $F = MA$, the terms involving $\mathbf{R}$ cancel:
$$\sum\mathbf{r'}_j\times\mathbf{f}_j = \frac{d}{dt}(\sum\mathbf{r'}_j\times m_j\mathbf{\dot{r}'}_j)$$
$$\mathbf{L}_{cm} = \sum\mathbf{r'}_j\times m_j\mathbf{\dot{r}'}_j$$
so, how can we then express $\mathbf{L}_{cm}$ in terms of its instantaneous angular velocity $\omega$? 
the length of $\mathbf{r}_j$ is fixed, but not the direction:
$$\mathbf{\dot{r}'}_j = \omega\times\mathbf{r'}_j$$
and $$\mathbf{L}_{cm} = \sum\mathbf{r'}_j\times m_j(\omega\times\mathbf{r'}_j)$$
we can then shed the extra notation by adopting center of mass coordinates:
$$\mathbf{L}=\sum\mathbf{r}_j\times m_j(\omega\times\mathbf{r}_j)$$
%% we will call this equation 4%%

we can then evaluate the cross products using Cartesian coordinates, which produces:
$$L_x = \sum m_j(y_j^2 + z_j^2)\omega_x - \sum m_jx_j\omega_y - \sum m_jx_jz_j\omega_z$$
if we introduce the following symbols:
$$I_{xx} = \sum m_j(y_j^2 + z_j^2)$$
$$I_{xy} = -\sum m_jx_jy_j$$
$$I_{xy} = -\sum m_jx_jz_j$$
$I_{xx}$ is called the moment of inertia, and is the same moment of inertia we introduced for **fixed axis rotation**
	aka $I = \sum m_j\rho_j^2$ where we take the axis in such a way that $\rho_j^2 = y_j^2 + z_j^2$
$I_{xy}$ and $I_{xz}$ are products of inertia, and are symmetrical in x and y

We then repeat the above derivation for $L_y$ and $L_z$:
$$L_x = I_{xx}\omega_x + I_{xy}\omega_y + I_{xz}\omega_z$$
$$L_y = I_{yx}\omega_x + I_{yy}\omega_y + I_{yz}\omega_z$$
$$L_z = I_{zx}\omega_x + I_{zy}\omega_y + I_{zz}\omega_z$$
these three equations then are able to describe rotation around any axes.
	fixed rotation is a special case-- rotation about an axis in the z direction, for example, has $\omega = \omega\mathbf{\hat{k}}$ and therefore, $L_z = I_{zz}\omega_z$
if the axis is not fixed, angular velocity about any coordinate axis will create angular momentum about any of the other coordinate axes.
Thus, as we have shown, $\mathbf{L}$ does not necessarily point in the same direction as $\mathbf{\omega}$.

[[example - rotating dumbell]]
but good news! since the above equations are wack, we can just write:
$$\mathbf{L} = \widetilde{\mathbf{I}}\mathbf{\omega}$$
Where $\widetilde{\mathbf{I}}$ is the tensor of inertia.
can also be represented as an array:
$$\mathbf{\widetilde{I}} = \left[\begin{array}{ccc}I_{xx}&I_{xy}&I_{xz} \\ I_{yx} & I_{yy} & I_{yz} \\ I_{zx} & I_{zy} & I_{zz}\end{array}\right]$$
Thus, $\mathbf{\widetilde{I}}\omega$ can also be represented through matrix multiplication, writing $\mathbf{L}$ and $\omega$ as column vectors.

## 8.6.2. principal axes
if the symmetry axes coincide with the coordinate axes, the tensor of inertia becomes quite simple:
$$\mathbf{\widetilde{I}} = \left(\begin{matrix}I_{xx} & 0 & 0 \\ 0 & I_{yy} & 0 \\ 0 & 0 & I_{zz}\end{matrix}\right)$$
for a body of any shape and mass distribution, it is actually possible to find a set of three perpendicular axes in which the products of inertia vanish!
- these axes are known as **principal axes**

thus, suppose we introduce a coordinate system 1, 2, 3 coinciding with the principal axes:
$$L_1 = I_1\omega_1$$
$$L_2 = I_2\omega_2$$
$$L_3 = I_3\omega_3$$

## 8.6.3 rotational kinetic energy of a rigid body
kinetic energy of a rigid body, including translational and rotational:
$$K = \frac{1}{2}\sum m_jv_j^2$$
$$\mathbf{r}_j = \mathbf{R} + \mathbf{r'}_j$$
$$\mathbf{v_j} = \mathbf{V} + \mathbf{v'}_j$$
And thus
$$K = \frac{1}{2}MV^2 + \frac{1}{2}\sum m_jv_j^2$$
using $\mathbf{v'}_j = \omega\times\mathbf{r'}_j$:
$$K_{rot} = \frac{1}{2}\sum m_j(\omega\times\mathbf{r'}_j)\cdot(\omega\times\mathbf{r'}_j)$$
and using the vector identity $(\mathbf{A}\times\mathbf{B})\cdot\mathbf{C}=\mathbf{A}\cdot(\mathbf{B}\times\mathbf{C})$
$$K_{rot} = \frac{1}{2}\omega\cdot[\sum m_j\mathbf{r'}_j\times(\omega\times\mathbf{r'}_j)]$$
and $$K_{rot} = \frac{1}{2}\omega\cdot\mathbf{L}$$
So, when $\omega$ and $\mathbf{L}$ are referred to principal axes:
$$K_{rot} = \frac{1}{2}I_1\omega_1^2 + \frac{1}{2}I_2\omega_2^2 + \frac{1}{2}I_3\omega_3^2$$
And thus
$$K_{rot} = \frac{L_1^2}{2I_1} + \frac{L_2^2}{2I_2} + \frac{L_3^2}{2I_3}$$
[[flying saucer vs flying cigar]]

## 8.6.4 rotation about a fixed point

if one point of the body is fixed, it is often convenient to analyze it as if that point were the origin
so, take a particle of mass $m_j$ and position vector of $\mathbf{r}_j$
$\mathbf{R} = X\mathbf{\hat{i}} + \mathbf{Y\hat{j}} + \mathbf{Z\hat{k}}$ is the position vector of the center of mass
Thus, the torque around the origin:
$$\tau = \sum r_j\times f_j$$
We can use the tensor of inertia, but we have to recalibrate for the moved origin--the original equations used prime to indicate center of mass coordinates

If we know $\mathbf{\widetilde{I}}_0$, then we can know $\mathbf{\widetilde{I}}$ about any other origin via the generalization of the parallel axis theorem

generally:
$$I_{xx} = (I_0)_{xx} + M(Y^2 + Z^2)$$
$$I_{xy} = (I_0)_{xy} - MXY$$
