added complexity via two harmonic oscillators:
	if the oscillators interact even slightly, the system acquires unique properties

consider a system of two identical pendulums of length $l$ and mass $m$, described by angles $\theta_1$ and $\theta_2$.
![[Pasted image 20251013162427.png]]
thus, the equations of motion are:
$$ml\ddot{\theta_1} = -lmg\theta_1$$
$$ml\ddot{\theta}_2 = -lmg\theta_2$$
when apart, these pendulums individually follow their motion. however, when connected by a weak spring of constant $k,$ the equations of motion change:
$$ml\ddot{\theta_1} = -lmg\theta_1 - ks(\theta_1 - \theta_2)$$
$$ml\ddot{\theta}_2 = -lmg\theta_2 + ks(\theta_1 - \theta_2)$$
using $\omega_0^2 = g/l$, $\kappa^2 = ks/ml$ and $\Omega^2 = \omega_0^2 + \kappa^2$, 
$$\ddot{\theta_1} + \Omega^2\theta_1 = \kappa^2\theta_2$$
$$\ddot{\theta}_2 + \Omega^2\theta_2 = \kappa^2\theta_1$$
we can assume that the motions are periodic, and such:
$$\theta_1(t) = A_1\sin(\omega t + \phi)$$
$$\theta_2(t) = A_2\sin(\omega t + \phi)$$
if $\theta_1$ and $\theta_2$ differed in time dependence, the earlier equations would not align.
thus, with substitution:
$$(\Omega^2 - \omega^2)A = \kappa^2B$$
$$(\Omega^2 - \omega^2)B = \kappa^2A$$
and there are two possibilities for $\omega$:
$$\omega_0^2 + \kappa^2 - \omega^2 = \kappa^2$$
$$\omega_0^2+\kappa^2-\omega^2 = -\kappa^2$$
there are then two solutions for $\omega^2$:
$$\omega_+^2 = \omega_0^2 + 2\kappa^2$$
$$\omega_-^2 = \omega_0^2$$
so either $A = -B$ or $A = B$
the pendulums will either swing in opposite directions with the same amplitudes or the pendulums will swing together (in this case, the spring is never stretched).
these two possibilities are known as **normal modes**:
	a normal mode is a new oscillator with a unique frequency.

**mode 1**: frequency $\omega_+ = \sqrt{\omega_0^2 + 2\kappa^2x}, \theta_1 = -\theta_2$
	$\theta_1(t) = A_+\sin(\omega_+t+\phi_+)$
	$\theta_2(t) = -A_+\sin(\omega_+t + \phi_+)$

**mode 2**: frequency $\omega_- = \omega_0, \theta_1 = \theta_2$
	$\theta_1(t) = A_-\sin(\omega_-t+ \phi_-)$
	$\theta_2(t) = A_-\sin(\omega_-t+\phi_-)$

the most general possible motion of the system:
$$\theta_1(t) = A_+\sin\omega_+(t+\phi_+) + A_-\sin\omega_-(t+\phi_-)$$
$$\theta_2(t) = -A_+\sin\omega_-(t+\phi_+) + A_-\sin\omega_-(t+\phi_-)$$
